int fix

Foundation/Propositional/Kripke/Hilbert/Cl.lean
@@ -5,17 +5,39 @@ import Foundation.Propositional.Kripke.AxiomLEM
 namespace LO.Propositional
 
 open Kripke
+open Hilbert.Kripke
 open Formula.Kripke
 
-open Kripke
+namespace Kripke.FrameClass
+
+protected abbrev euclidean : FrameClass := { F | Euclidean F }
+
+namespace euclidean
+
+@[simp]
+instance nonempty : FrameClass.euclidean.Nonempty := by
+  use whitepoint;
+  simp [Euclidean];
+
+lemma validates_AxiomLEM : FrameClass.euclidean.ValidatesFormula (Axioms.LEM (.atom 0)) := by
+  rintro F _ _ rfl;
+  apply validate_LEM_of_euclidean $ by assumption
+
+instance validate_HilbertLC : FrameClass.euclidean.Validates (Hilbert.Cl.axioms) := by
+  apply FrameClass.Validates.withAxiomEFQ;
+  apply validates_AxiomLEM;
+
+end euclidean
+
+end Kripke.FrameClass
+
 
 namespace Hilbert.Cl.Kripke
 
-instance : FrameClass.euclidean.DefinedBy (Hilbert.Cl.axioms) := FrameClass.definedBy_with_axiomEFQ inferInstance
+instance sound : Sound Hilbert.Cl FrameClass.euclidean :=
+  instSound_of_validates_axioms FrameClass.euclidean.validate_HilbertLC
 
-instance sound : Sound Hilbert.Cl FrameClass.euclidean := inferInstance
-
-instance consistent : Entailment.Consistent Hilbert.Cl := Kripke.Hilbert.consistent_of_FrameClass FrameClass.euclidean (by simp)
+instance consistent : Entailment.Consistent Hilbert.Cl := consistent_of_sound_frameclass FrameClass.euclidean (by simp)
 
 instance canonical : Canonical Hilbert.Cl FrameClass.euclidean := ⟨Canonical.euclidean⟩
 
